Instantiate IRExpr

Semantics/RewriteTerms.thy
@@ -1,8 +1,5 @@
 theory RewriteTerms
-imports IRTreeEval Stratego.CompileRewrite
-begin
-                              
-instantiation IRExpr :: Rewritable
+imports IRTreeEval Stratego.CompileRewrite "HOL-Library.Monad_Syntax"
 begin
 
 fun rewrite_IRExpr :: "(IRExpr \<Rightarrow> IRExpr) \<Rightarrow> IRExpr \<Rightarrow> IRExpr" where
@@ -47,79 +44,280 @@ fun subexprs_IRExpr :: "IRExpr \<Rightarrow> IRExpr list" where
   "subexprs_IRExpr (ConditionalExpr c t f) = [c, t, f]" |
   "subexprs_IRExpr _ = []"
 
-fun chain_IRExpr :: "nat \<Rightarrow> (IRExpr \<Rightarrow> nat \<Rightarrow> (nat \<times> IRExpr)) \<Rightarrow> IRExpr \<Rightarrow> (nat \<times> IRExpr)" where
-  "chain_IRExpr n f (UnaryExpr op x) =
+fun chain_IRExpr :: "(IRExpr \<Rightarrow> nat \<Rightarrow> (nat \<times> IRExpr)) \<Rightarrow> IRExpr \<Rightarrow> nat \<Rightarrow> (nat \<times> IRExpr)" where
+  "chain_IRExpr f (UnaryExpr op x) n =
     (let (n', x') = f x n in
       (n', UnaryExpr op x'))" |
-  "chain_IRExpr n f (BinaryExpr op x y) =
+  "chain_IRExpr f (BinaryExpr op x y) n =
     (let (n', x') = f x n in
     (let (n'', y') = f y n' in
       (n'', BinaryExpr op x' y')))" |
-  "chain_IRExpr n f (ConditionalExpr c b1 b2) =
+  "chain_IRExpr f (ConditionalExpr c b1 b2) n =
     (let (n', c') = f c n in
     (let (n'', b1') = f b1 n' in
     (let (n''', b2') = f b2 n'' in
       (n''', ConditionalExpr c' b1' b2'))))" |
-  "chain_IRExpr n f e = (n, e)"
+  "chain_IRExpr f e n = (n, e)"
 
-(*instance proof qed*)
-instance proof
+
+datatype SideCondition =
+  IsConstantExpr IRExpr |
+  IsIntegerStamp IRExpr |
+  IsBoolStamp IRExpr |
+  WellFormed IRExpr |
+  IsStamp IRExpr Stamp |
+  IsConstantValue IRExpr IRExpr "64 word" |
+  AlwaysDistinct IRExpr IRExpr |
+  NeverDistinct IRExpr IRExpr |
+  StampUnder IRExpr IRExpr |
+  UpMaskEquals IRExpr "64 word" |
+  DownMaskEquals IRExpr "64 word" |
+  UpMaskCancels IRExpr IRExpr |
+  IsBool IRExpr |
+  PowerOf2 IRExpr |
+  Empty |
+  And SideCondition SideCondition |
+  Not SideCondition
+
+(*
+definition wf_stamp :: "IRExpr \<Rightarrow> bool" where
+  "wf_stamp e = (\<forall>m p v. ([m, p] \<turnstile> e \<mapsto> v) \<longrightarrow> valid_value v (stamp_expr e))"
+*)
+definition wf_stamp :: "IRExpr \<Rightarrow> bool" where
+  "wf_stamp e = False"
+fun eval_condition :: "SideCondition \<Rightarrow> bool" where
+  "eval_condition (IsConstantExpr e) = is_ConstantExpr e" |
+  "eval_condition (IsIntegerStamp e) = is_IntegerStamp (stamp_expr e)" |
+  "eval_condition (IsBoolStamp e) = (stamp_expr e = IntegerStamp 32 0 1)" |
+  "eval_condition (WellFormed e) = wf_stamp e" |
+  "eval_condition (IsStamp e s) = ((stamp_expr e) = s)" |
+  "eval_condition (IsConstantValue e s v) = (e = ConstantExpr (IntVal (stp_bits (stamp_expr s)) v))" |
+  "eval_condition (AlwaysDistinct e1 e2) = alwaysDistinct (stamp_expr e1) (stamp_expr e2)" |
+  "eval_condition (NeverDistinct e1 e2) = neverDistinct (stamp_expr e1) (stamp_expr e2)" |
+  "eval_condition (StampUnder e1 e2) = (stamp_under (stamp_expr e1) (stamp_expr e2))" |
+  "eval_condition (UpMaskEquals e m) = (IRExpr_up e = m)" |
+  "eval_condition (DownMaskEquals e m) = (IRExpr_down e = m)" |
+  "eval_condition (UpMaskCancels e1 e2) = (((and (IRExpr_up e1) (IRExpr_up e2)) = 0))" |
+  "eval_condition (PowerOf2 e) = False" |
+  "eval_condition (IsBool e) = ((e = ConstantExpr (IntVal 32 0)) | (e = ConstantExpr (IntVal 32 0)))" |
+  
+  "eval_condition (Empty) = True" |
+
+  "eval_condition (And sc1 sc2) = ((eval_condition sc1) \<and> (eval_condition sc2))" |
+  "eval_condition (Not sc) = (\<not>(eval_condition sc))"
+
+
+fun ground_expr :: "IRExpr \<Rightarrow> (string \<rightharpoonup> IRExpr) \<Rightarrow> IRExpr option" where
+  "ground_expr (UnaryExpr op e) s = do {
+    e <- ground_expr e s;
+    Some (UnaryExpr op e)
+  }" |
+  "ground_expr (BinaryExpr op e1 e2) s = do {
+    e1 <- ground_expr e1 s;
+    e2 <- ground_expr e2 s;
+    Some (BinaryExpr op e1 e2)
+  }" |
+  "ground_expr (ConditionalExpr b e1 e2) s = do {
+    b <- ground_expr b s;
+    e1 <- ground_expr e1 s;
+    e2 <- ground_expr e2 s;
+    Some (ConditionalExpr b e1 e2)
+  }" |
+  "ground_expr (VariableExpr vn st) s = 
+    (case s (String.explode vn) of None \<Rightarrow> None
+                | Some v' \<Rightarrow> Some v')" |
+  "ground_expr e s = Some e"
+
+lemma
+  assumes sub: "a' \<subseteq>\<^sub>m a"
+  assumes e': "ground_expr e a' = Some e'"
+  shows "ground_expr e a' = ground_expr e a"
+  using assms apply (induction e a' arbitrary: a a' rule: ground_expr.induct; auto)
+  sorry
+  
+
+fun ground_condition :: "SideCondition \<Rightarrow> (string \<rightharpoonup> IRExpr) \<Rightarrow> SideCondition option" where
+  "ground_condition (IsConstantExpr e) f = do {e <- ground_expr e f; Some (IsConstantExpr e)}" |
+  "ground_condition (IsIntegerStamp e) f = do {e <- ground_expr e f; Some (IsIntegerStamp e)}" |
+  "ground_condition (IsBoolStamp e) f = do {e <- ground_expr e f; Some (IsBoolStamp e)}" |
+  "ground_condition (WellFormed e) f = do {e <- ground_expr e f; Some (WellFormed e)}" |
+  "ground_condition (IsStamp e s) f = do {e <- ground_expr e f; Some (IsStamp e s)}" |
+  "ground_condition (IsConstantValue e s v) f = do {e <- ground_expr e f; Some (IsConstantValue e s v)}" |
+  "ground_condition (AlwaysDistinct e1 e2) f = do {
+    e1 <- ground_expr e1 f;
+    e2 <- ground_expr e2 f;
+    Some (AlwaysDistinct e1 e2)
+  }" |
+  "ground_condition (NeverDistinct e1 e2) f = do {
+    e1 <- ground_expr e1 f;
+    e2 <- ground_expr e2 f;
+    Some (NeverDistinct e1 e2)
+  }" |
+  "ground_condition (StampUnder e1 e2) f = do {
+    e1 <- ground_expr e1 f;
+    e2 <- ground_expr e2 f;
+    Some (StampUnder e1 e2)
+  }" |
+  "ground_condition (UpMaskEquals e m) f = 
+    do {e <- ground_expr e f; Some (UpMaskEquals e m)}" |
+  "ground_condition (DownMaskEquals e m) f = 
+    do {e <- ground_expr e f; Some (DownMaskEquals e m)}" |
+  "ground_condition (UpMaskCancels e1 e2) f = do {
+    e1 <- ground_expr e1 f;
+    e2 <- ground_expr e2 f;
+    Some (UpMaskCancels e1 e2)
+  }" |
+  "ground_condition (PowerOf2 e) f = do {e <- ground_expr e f; Some (PowerOf2 e)}" |
+  "ground_condition (IsBool e) f = do {e <- ground_expr e f; Some (IsBool e)}" |
+  
+  "ground_condition (Empty) f = Some (Empty)" |
+
+  "ground_condition (And sc1 sc2) f = do {
+    sc1 <- ground_condition sc1 f;
+    sc2 <- ground_condition sc2 f;
+    Some (And sc1 sc2)
+  }" |
+  "ground_condition (Not sc) f = do {
+    sc <- ground_condition sc f;
+    Some (Not sc)
+  }"
+
+datatype Result =
+  ExpressionResult IRExpr |
+  forZero IRExpr |
+  Negate IRExpr |
+  Add IRExpr IRExpr
+
+fun result_of :: "Result \<Rightarrow> IRExpr" where
+  "result_of (ExpressionResult e) = e" |
+  "result_of (forZero e) = ConstantExpr (IntVal (stp_bits (stamp_expr e)) 0)" |
+  "result_of (Negate (ConstantExpr (IntVal b v))) = ConstantExpr (intval_negate (IntVal b v))" |
+  "result_of (Add (ConstantExpr (IntVal b1 v1)) (ConstantExpr (IntVal b2 v2))) = ConstantExpr (intval_add (IntVal b1 v1) (IntVal b2 v2))" 
+
+fun ground_result :: "Result \<Rightarrow> (string \<rightharpoonup> IRExpr) \<Rightarrow> Result option" where
+  "ground_result (ExpressionResult e) s = do {e <- ground_expr e s; Some (ExpressionResult e)}" |
+  "ground_result (forZero e) s = do {e <- ground_expr e s; Some (forZero e)}" |
+  "ground_result (Negate e) s = do {e <- ground_expr e s; Some (Negate e)}" |
+  "ground_result (Add e1 e2) s = do {
+    e1 <- ground_expr e1 s;
+    e2 <- ground_expr e2 s;
+    Some (Add e1 e2)
+  }"
+
+setup \<open>Locale_Code.open_block\<close>
+interpretation IRExprRewrites : Rewritable
+  size_IRExpr
+  "eval_condition"
+  "ground_condition"
+  result_of
+  ground_result
+  rewrite_IRExpr
+  match_IRExpr
+  varof_IRExpr
+  var_IRExpr
+proof
+  fix a' a :: "(string \<rightharpoonup> IRExpr)"
+  fix e e' :: SideCondition
+  assume sub: "a' \<subseteq>\<^sub>m a"
+  assume e': "ground_condition e a' = Some e'"
+  show "ground_condition e a' = ground_condition e a"
+    using sub e' apply (induction e a' arbitrary: a a' rule: ground_condition.induct; auto)
+    sorry
+qed
+setup \<open>Locale_Code.close_block\<close>
+
+setup \<open>Locale_Code.open_block\<close>
+interpretation IRExprRewrites: CompiledRewrites
+  size_IRExpr
+  "eval_condition"
+  "ground_condition"
+  result_of
+  ground_result
+  rewrite_IRExpr
+  match_IRExpr
+  varof_IRExpr
+  var_IRExpr
+  subexprs_IRExpr
+  chain_IRExpr
+proof
   fix e :: IRExpr
-  show "\<forall>e' \<in> set (subexprs e). size e > size e'"
+  show "\<forall>e' \<in> set (subexprs_IRExpr e). size_IRExpr e > size_IRExpr e'"
     by (cases e; simp)
 next
   fix f :: "IRExpr \<Rightarrow> IRExpr"
   fix e :: IRExpr
-  show "map f (subexprs e) = subexprs (snd (chain 0 (\<lambda>e a. (plus a 1, f e)) e))"
+  show "map f (subexprs_IRExpr e) = subexprs_IRExpr (snd (chain_IRExpr (\<lambda>e a. (plus a 1, f e)) e 0))"
     by (cases e; simp)
 next
   fix f :: "IRExpr \<Rightarrow> IRExpr"
   fix e :: IRExpr
-  show "length (subexprs e) = fst (chain 0 (\<lambda>e a. (plus a 1, f e)) e)"
+  show "length (subexprs_IRExpr e) = fst (chain_IRExpr (\<lambda>e a. (plus a 1, f e)) e 0)"
     by (cases e; simp)
 qed
-end
+setup \<open>Locale_Code.close_block\<close>
 
-definition RedundantAdd :: "IRExpr Strategy" where
+definition eval where "eval = IRExprRewrites.eval"
+definition var where "var = var_IRExpr"
+
+no_notation Arithmetic.func ("func _")
+no_notation Arithmetic.else ("_ else _")
+notation IRExprRewrites.conditional_rewrite_to ("_ \<rightarrow> _ where _")
+notation IRExprRewrites.not ("not _")
+notation IRExprRewrites.condition ("condition _")
+notation IRExprRewrites.func ("func _")
+
+type_synonym StrategyRule = "(IRExpr, SideCondition, Result) IRExprRewrites.Strategy"
+
+code_datatype fmap_of_list
+lemma fmlookup_of_list[code]: "fmlookup (fmap_of_list m) = map_of m"
+  by (simp add: fmlookup_of_list)
+
+export_code "eval" checking SML
+
+definition join where "join = IRExprRewrites.join"
+definition compile' where "compile' = IRExprRewrites.compile'"
+definition generate where "generate = IRExprRewrites.generate"
+definition generate_with_condition where "generate_with_condition = IRExprRewrites.generate_with_condition"
+
+definition match_pattern where "match_pattern = IRExprRewrites.match_pattern"
+definition optimized_export where "optimized_export = IRExprRewrites.optimized_export"
+notation IRExprRewrites.choice ("choice _")
+notation IRExprRewrites.else ("_ else _")
+
+export_code "compile'" checking SML
+
+definition RedundantAdd :: "StrategyRule" where
   "RedundantAdd = 
     ((BinaryExpr BinAdd (var ''b'') (ConstantExpr (IntVal 32 0))) 
       \<rightarrow> (var ''b''))"
 
-definition RedundantSub :: "IRExpr Strategy" where
+definition RedundantSub :: "StrategyRule" where
   "RedundantSub = 
     ((BinaryExpr BinSub (var ''a'') (ConstantExpr (IntVal 32 0)))
       \<rightarrow> (var ''a''))"
 
-definition ShiftConstRight :: "IRExpr Strategy" where
+definition ShiftConstRight :: "StrategyRule" where
   "ShiftConstRight = 
     ((BinaryExpr BinAdd (var ''a'') (var ''b'')) \<rightarrow> (BinaryExpr BinAdd (var ''b'') (var ''a''))
       where ((var ''a'')!; not (ConstantExpr (IntVal 32 0)?)))"
 
-fun negate :: "IRExpr \<Rightarrow> IRExpr" where
-  "negate (ConstantExpr v) = (ConstantExpr (intval_negate v))" |
-  "negate x = x"
-
-definition EvalMinus :: "IRExpr Strategy" where
+definition EvalMinus :: "StrategyRule" where
   "EvalMinus = 
     ((UnaryExpr UnaryNeg (var ''a'')) \<rightarrow> ((var ''b''))
-      where (<is_ConstantExpr>?(var ''a''); ((var ''a'')!; func negate); (var ''b'')?))"
+      where (condition (IsConstantExpr (var ''a'')); (func (Negate (var ''a''))); (var ''b'')?))"
 
-definition EvalMinus1 :: "IRExpr Strategy" where
+definition EvalMinus1 :: "StrategyRule" where
   "EvalMinus1 =
     (UnaryExpr UnaryNeg (var ''a'')) \<rightarrow> var ''b''
-      where (<is_ConstantExpr>?(var ''a''); (var ''b'') := (<negate>(var ''a'')))"
+      where (condition (IsConstantExpr (var ''a'')); (var ''b'') := (func Negate (var ''a'')))"
 
-fun add :: "IRExpr \<Rightarrow> IRExpr" where
-  "add (BinaryExpr BinAdd (ConstantExpr v1) (ConstantExpr v2)) = (ConstantExpr (intval_add v1 v2))" |
-  "add x = x"
-
-definition EvalAdd :: "IRExpr Strategy" where
+definition EvalAdd :: "StrategyRule" where
   "EvalAdd =
     (BinaryExpr BinAdd (var ''a'') (var ''b'')) \<rightarrow> ((var ''c''))
       where (
-        <is_ConstantExpr>?(var ''a'');
-        <is_ConstantExpr>?(var ''b'');
-        (var ''c'') := <add>(BinaryExpr BinAdd (var ''a'') (var ''b''))
+        condition (IsConstantExpr (var ''a''));
+        condition (IsConstantExpr (var ''b''));
+        (var ''c'') := func (Add (var ''a'') (var ''b''))
       )"
 
 value "eval (RedundantAdd <+ RedundantSub)
@@ -133,7 +331,7 @@ value "eval (RedundantAdd <+ RedundantSub)
 value "eval (RedundantSub <+ RedundantAdd)
         ((BinaryExpr BinAdd (ConstantExpr (IntVal 32 10)) (ConstantExpr (IntVal 32 0))), fmempty)"
 
-value "ShiftConstRight"
+(*value "ShiftConstRight"*)
 value "eval ShiftConstRight 
       ((BinaryExpr BinAdd (ConstantExpr (IntVal 32 10)) (ConstantExpr (IntVal 32 0))), fmempty)"
 value "eval ShiftConstRight
@@ -146,23 +344,46 @@ value "eval EvalMinus ((UnaryExpr UnaryNeg (BinaryExpr BinAdd (ConstantExpr (Int
 value "eval EvalAdd ((UnaryExpr UnaryNeg (ConstantExpr (IntVal 32 10))), fmempty)"
 value "eval EvalAdd ((BinaryExpr BinAdd (ConstantExpr (IntVal 32 10)) (ConstantExpr (IntVal 32 10))), fmempty)"
 
-value "(choice [compile' RedundantAdd, compile' RedundantSub])"
-value "(optimized_export (choice [compile' RedundantAdd, compile' RedundantSub]))"
+
+instantiation IRExpr :: full_exhaustive
+begin
+instance ..
+end
+
+instantiation SideCondition :: full_exhaustive
+begin
+instance ..
+end
+
+instantiation Result :: full_exhaustive
+begin
+instance ..
+end
+
+lemma exhaust_SideCondition[code]:
+"full_exhaustive_SideCondition_inst.full_exhaustive_SideCondition f d = None"
+  sorry
+lemma exhaust_Result[code]:
+"full_exhaustive_Result_inst.full_exhaustive_Result f d = None"
+  sorry
+lemma exhaust_IRExpr[code]:
+"full_exhaustive_IRExpr_inst.full_exhaustive_IRExpr f d = None"
+  sorry
+
+value "RedundantAdd"
+value "(choice [the (compile' RedundantAdd), the (compile' RedundantSub)])"
+value "(optimized_export (choice [the (compile' RedundantAdd), the (compile' RedundantSub)]))"
 
 
 
 
 text \<open>@{text "x * const 1 \<longrightarrow> x"}\<close>
-fun alwaysTrue :: "IRExpr \<Rightarrow> bool" where
-  "alwaysTrue e = True"
-
 definition Identity where
   "Identity = generate 
     (BinaryExpr BinMul
       (var ''x'')
       (ConstantExpr (IntVal 32 1)))
-    (var ''x'')
-    (var ''x'', alwaysTrue)"
+    (var ''x'')"
 
 value "Identity"
 value "(optimized_export (Identity))"
@@ -173,15 +394,14 @@ definition Evaluate where
     (BinaryExpr BinMul
       (ConstantVar STR ''x'')
       (ConstantVar STR ''y''))
-    ((ConstantVar STR ''x''))
-    (var ''x'', alwaysTrue)"
+    ((ConstantVar STR ''x''))"
 (* doesn't support constant evaluation *)
 value "Evaluate"
 value "(optimized_export (Evaluate))"
 
 text \<open>@{text "x * const y \<longrightarrow> x << const (log2 y)"}\<close>
 definition Shift where
-  "Shift = generate 
+  "Shift = generate_with_condition 
     (BinaryExpr BinMul
       (var ''x'')
       (ConstantVar STR ''y''))
@@ -193,17 +413,18 @@ value "Shift"
 
 text \<open>@{text "const x * y \<longrightarrow> y * const x when NotConst y"}\<close>
 definition LeftConst where
-  "LeftConst = generate 
+  "LeftConst = generate_with_condition 
     (BinaryExpr BinMul
       (ConstantVar STR ''x'')
       (var ''y''))
-    (ExpressionResult (BinaryExpr BinMul (var ''y'') (ConstantVar STR ''x'')))
+    ((BinaryExpr BinMul (var ''y'') (ConstantVar STR ''x'')))
     (Not (IsConstantExpr (var ''y'')))"
 (* doesn't support constant evaluation *)
 value "LeftConst"
 
+(*no_notation "\<^syntax_const>\<open>_thenM\<close>" (infixl "\<then>" 54)*)
 
-value "(optimized_export (optimized_export (LeftConst \<then> (Evaluate else (Identity else Shift)))))"
+value "LeftConst else Evaluate else Identity else Shift"
 
 
 end
